vtr/coq/lib/Semantics/PolyTyp.v
@@ -1,0 +1,105 @@
+Require Export CoqRecon.Util.ListEnv CoqRecon.Semantics.DeclTyping.
+
+(** Poly-types/type-schemes. *)
+Record poly : Set :=
+  { pvars : list nat; ptyp : typ }.
+
+Definition pgamma : Set := list (string * poly).
+
+Declare Scope poly_scope.
+Delimit Scope poly_scope with poly.
+
+Notation "∀ X , t"
+  := ({| pvars := X; ptyp := t |})
+       (at level 50, no associativity) : poly_scope.
+
+Open Scope poly_scope.
+Open Scope set_scope.
+
+Definition ptvars (p : poly) : list nat := tvars (ptyp p) ∖ pvars p.
+
+Definition ftv : pgamma -> list nat :=
+  fold_right (fun '(x,p) => app (ptvars p)) [].
+
+Definition pnv (t : typ) : poly :=
+  {| pvars := []; ptyp := t |}.
+
+Coercion pnv : typ >-> poly.
+
+(** Alpha equivalence of [poly] *)
+Definition alpha (p1 p2 : poly) : Prop :=
+  satisfy ([[ pvars p1 ⟼  map TVar (pvars p2) ]]) (ptyp p1) (ptyp p2).
+
+Notation "p1 ≂ p2"
+  := (alpha p1 p2)
+       (at level 70, no associativity) : type_scope.
+
+Section Alpha.
+  Local Hint Resolve satisfy_reflexive : core.
+
+  Lemma alpha_reflexive : Reflexive alpha.
+  Proof.
+    intuition.
+  Qed.
+
+  Local Hint Resolve satisfy_symmetric : core.
+  Local Hint Unfold alpha : core.
+  Local Hint Unfold Symmetric : core.
+  
+  Lemma alpha_symmetric : Symmetric alpha.
+  Proof.
+    autounfold with core.
+    intros [XS x] [YS y] Hxy; simpl in *.
+    symmetry.
+  Abort.
+
+  Local Hint Resolve satisfy_transitive : core.
+  Local Hint Unfold Transitive : core.
+  
+  Lemma alpha_transitive : Transitive alpha.
+  Proof.
+    autounfold with core.
+    intros [XS x] [YS y] [ZS z] Hxy Hyz; simpl in *.
+  Abort.
+End Alpha.
+
+Reserved Notation "g ⫢ e ∴ p"
+         (at level 70, no associativity).
+
+Open Scope term_scope.
+
+(** Damas Milner Declarative-typing system. *)
+Inductive DM (Γ : pgamma) : term -> poly -> Prop :=
+| DM_var x p :
+    lookup x Γ = Some p ->
+    Γ ⫢ x ∴ p
+| DM_abs x e (τ τ' : typ) :
+    ((x, pnv τ) :: Γ) ⫢ e ∴ τ' ->
+    Γ ⫢ λ x ⇒ e ∴ τ → τ'
+| DM_app e1 e2 (τ τ' : typ) :
+    Γ ⫢ e1 ∴ τ → τ' ->
+    Γ ⫢ e2 ∴ τ ->
+    Γ ⫢ e1 ⋅ e2 ∴ τ'
+| DM_let x e1 e2 p (τ : typ) :
+    Γ ⫢ e1 ∴ p ->
+    ((x, p) :: Γ) ⫢ e2 ∴ τ ->
+    Γ ⫢ LetIn x e1 e2 ∴ τ
+| DM_gen e XS (τ : typ) :
+    Disjoint XS (ftv Γ) ->
+    Γ ⫢ e ∴ τ ->
+    Γ ⫢ e ∴ ∀ XS, τ
+| DM_inst e (τ : typ) XS TS :
+    Γ ⫢ e ∴ (∀ XS, τ) ->
+    Γ ⫢ e ∴ [[ XS ⟼  TS ]] † τ
+| DM_cond e1 e2 e3 p p' :
+    p ≂ p' ->
+    Γ ⫢ e1 ∴ TBool ->
+    Γ ⫢ e2 ∴ p ->
+    Γ ⫢ e3 ∴ p' ->
+    Γ ⫢ Cond e1 e2 e3 ∴ p
+| DM_op o e1 e2 τ τ' :
+    op_typs o τ τ' ->
+    Γ ⫢ e1 ∴ τ ->
+    Γ ⫢ e2 ∴ τ ->
+    Γ ⫢ Op o e1 e2 ∴ τ'
+where "g ⫢ e ∴ p" := (DM g e p) : type_scope.
