vtr/coq/lib/Util/ListEnv.v
@@ -1,0 +1,107 @@
+Require Export Coq.Classes.EquivDec
+        CoqRecon.Util.Sets CoqRecon.Util.Maybe
+        CoqRecon.Util.Env.
+
+Open Scope env_scope.
+
+Section Lookup.
+  Context {K V : Set} {HDK : EqDec K eq}.
+
+  Fixpoint lookup (k : K) (l : list (K * V)) : option V :=
+    match l with
+    | []         => None
+    | (k',v) :: l => if k == k' then Some v else lookup k l
+    end.
+  
+  Definition to_env : list (K * V) -> @env K V :=
+    fold_right (uncurry bind) ∅.
+
+  Definition combine_to_env (ks : list K) (vs : list V) : @env K V :=
+    to_env (combine ks vs).
+  
+  Definition eql (l1 l2 : list (K * V)) : Prop :=
+    forall k, lookup k l1 = lookup k l2.
+
+  Definition env_eq (l : list (K * V)) (e : @env K V) : Prop :=
+    forall k, lookup k l = e k.
+End Lookup.
+
+Notation "l1 ≊ l2"
+  := (eql l1 l2)
+       (at level 70, no associativity) : type_scope.
+
+Notation "l ⩰ e"
+  := (env_eq l e)
+       (at level 70, no associativity) : type_scope.
+
+Notation "'[[' ks ⟼  vs ']]'"
+  := (combine_to_env ks vs)
+       (at level 10, no associativity) : env_scope.
+
+Section Env.
+  Context {K V : Set} {HDK : EqDec K eq}.
+  
+  Lemma cons_env_sound : forall (k : K) (v : V) (l : list (K * V)),
+      lookup k ((k,v) :: l) = Some v.
+  Proof.
+    intros k v l; simpl.
+    dispatch_eqdec; auto.
+  Qed.
+
+  Lemma cons_env_complete : forall (x k : K) (v : V) (l : list (K * V)),
+      x <> k -> lookup x ((k,v) :: l) = lookup x l.
+  Proof.
+    intros x k v l Hxk; simpl.
+    dispatch_eqdec; auto.
+  Qed.
+
+  Local Hint Unfold eql : core.
+  
+  Lemma cons_env_same : forall (k : K) (v v' : V) (l : list (K * V)),
+      (k,v) :: (k,v') :: l ≊ (k,v) :: l.
+  Proof.
+    intros k v v' l k'; simpl;
+      repeat dispatch_eqdec; auto.
+  Qed.
+
+  Lemma cons_env_diff_comm : forall (x y : K) (u v : V) (l : list (K * V)),
+      x <> y -> (x,u) :: (y,v) :: l ≊ (y,v) :: (x,u) :: l.
+  Proof.
+    intros x y u v l Hxy k; simpl;
+      repeat dispatch_eqdec; auto.
+  Qed.
+  
+  Lemma to_env_sound : forall l : list (K * V),
+      l ⩰ to_env l.
+  Proof.
+    unfold to_env, "⩰", "∅".
+    intro l; induction l as [| [k v] l IHl];
+      intro k'; simpl; auto.
+    unfold bind at 1.
+    dispatch_eqdec; auto.
+  Qed.
+  
+  Lemma to_env_eql : forall l l' : list (K * V),
+      l ≊ l' -> to_env l = to_env l'.
+  Proof.
+    unfold "≊", to_env, "∅".
+    intro l; induction l as [| [k v] l IHl];
+      intros [| [k' v'] l'] Heql;
+      extensionality x;
+      specialize Heql with x as Heql';
+      simpl in *; try unfold bind at 1;
+        repeat dispatch_eqdec; auto.
+    - rewrite Heql' at 1. apply to_env_sound.
+    - symmetry. rewrite <- Heql' at 1.
+      apply to_env_sound.
+    - rewrite bind_sound. assumption.
+    - rewrite bind_complete by assumption.
+      rewrite Heql'. apply to_env_sound.
+    - rewrite bind_sound. symmetry.
+      rewrite <- Heql'. apply to_env_sound.
+    - rewrite bind_complete by assumption.
+      apply equal_f; apply IHl.
+      intro y; specialize Heql with y.
+      repeat dispatch_eqdec; auto.
+  Abort.
+End Env.
